substitution, beta-reduction, and the type-preservation property

src/PreSimplyTyped.thy
@@ -1,5 +1,5 @@
 theory PreSimplyTyped
-imports Main Permutation
+imports Main Fresh Permutation
 begin
 
 type_synonym tvar = nat
@@ -476,6 +476,7 @@ corollary ptrm_alpha_equiv_transp:
   shows "transp ptrm_alpha_equiv"
 unfolding transp_def using ptrm_alpha_equiv_transitive by auto
 
+
 type_synonym 'a typing_ctx = "'a \<rightharpoonup> type"
 
 fun ptrm_infer_type :: "'a typing_ctx \<Rightarrow> 'a ptrm \<Rightarrow> type option" where
@@ -656,5 +657,106 @@ using assms proof(induction arbitrary: \<Gamma>, simp, simp, simp)
     thus ?case by simp
   next
 qed
+
+context fresh
+begin
+
+function ptrm_subst :: "'a ptrm \<Rightarrow> 'a \<Rightarrow> 'a ptrm \<Rightarrow> 'a ptrm" where
+  "ptrm_subst (PVar x)    z M = (if x = z then M else PVar x)"
+| "ptrm_subst (PApp A B)  z M = PApp (ptrm_subst A z M) (ptrm_subst B z M)"
+| "ptrm_subst (PFn x T A) z M =
+     (if x = z
+        then PFn x T A
+        else (let
+          y = fresh_in ({z} \<union> ptrm_fvs A \<union> ptrm_fvs M) in
+          PFn y T (ptrm_subst ([x \<leftrightarrow> y] \<bullet> A) z M)))"
+by (pat_completeness, auto)
+termination by(relation "measure (size \<circ> fst)", auto, metis ptrm_size_prm lessI)
+
+lemma ptrm_subst_alpha_equiv_left:
+  assumes "X \<approx> Y"
+  shows "ptrm_subst X z M \<approx> ptrm_subst Y z M"
+sorry
+
+(*
+using assms proof(induction "size X" arbitrary: X Y rule: less_induct)
+  fix X Y :: "'a ptrm"
+  assume IH: "\<And>K J. \<lbrakk>size K < size X; K \<approx> J\<rbrakk> \<Longrightarrow> ptrm_subst K z M \<approx> ptrm_subst J z M"
+  and "X \<approx> Y"
+
+  show "ptrm_subst X z M \<approx> ptrm_subst Y z M"
+  using `X \<approx> Y` IH proof(induction rule: ptrm_alpha_equiv.induct)
+    case (fn1 A B x T)
+      consider "z = x" | "z \<noteq> x" by auto
+      thus ?case proof(cases)
+        case 1
+          thus ?thesis using fn1 ptrm_alpha_equiv.fn1 ptrm_subst.simps(3) by fastforce
+        next
+        case 2
+          obtain y1 where y1: "y1 = fresh_in({z} \<union> ptrm_fvs A \<union> ptrm_fvs M)" by auto
+          hence *: "ptrm_subst (PFn x T A) z M = PFn y1 T (ptrm_subst ([x \<leftrightarrow> y1] \<bullet> A) z M)"
+            using `z \<noteq> x` ptrm_subst.simps(3) by metis
+
+          obtain y2 where y2: "y2 = fresh_in({z} \<union> ptrm_fvs B \<union> ptrm_fvs M)" by auto
+          hence **: "ptrm_subst (PFn x T B) z M = PFn y2 T (ptrm_subst ([x \<leftrightarrow> y2] \<bullet> B) z M)"
+            using `z \<noteq> x` ptrm_subst.simps(3) by metis
+
+          have "ptrm_fvs A = ptrm_fvs B" using `A \<approx> B` ptrm_alpha_equiv_fvs by metis
+          hence "y1 = y2" using y1 y2 by auto
+          hence "[x \<leftrightarrow> y1] \<bullet> A \<approx> [x \<leftrightarrow> y2] \<bullet> B" using `A \<approx> B` ptrm_alpha_equiv_prm by metis
+
+          have "size ([x \<leftrightarrow> y1] \<bullet> A) = size A"
+            using ptrm_size_prm by metis
+          hence "size ([x \<leftrightarrow> y1] \<bullet> A) < size (PFn x T A)" by auto
+
+          hence "ptrm_subst ([x \<leftrightarrow> y1] \<bullet> A) z M \<approx> ptrm_subst ([x \<leftrightarrow> y2] \<bullet> B) z M"
+            using fn1.prems `[x \<leftrightarrow> y1] \<bullet> A \<approx> [x \<leftrightarrow> y2] \<bullet> B` by metis
+          thus ?thesis using * ** `y1 = y2` ptrm_alpha_equiv.fn1 by metis
+        next
+      qed
+    next
+    case (fn2 a b A B T)
+      thus ?case
+*)
+
+lemma ptrm_subst_alpha_equiv_right:
+  assumes "M \<approx> N"
+  shows "ptrm_subst X z M \<approx> ptrm_subst X z N"
+using assms proof(induction "size X" arbitrary: X M N rule: less_induct)
+  fix X M N :: "'a ptrm"
+  assume "\<And>K M N. \<lbrakk>size K < size X; M \<approx> N\<rbrakk> \<Longrightarrow> ptrm_subst K z M \<approx> ptrm_subst K z N"
+  and "M \<approx> N"
+  hence IH: "\<And>K. size K < size X \<Longrightarrow> ptrm_subst K z M \<approx> ptrm_subst K z N" by metis
+
+  show "ptrm_subst X z M \<approx> ptrm_subst X z N"
+  proof(cases X)
+    case (PVar x)
+      thus ?thesis by(cases "x = z", auto simp add: `M \<approx> N` ptrm_alpha_equiv_reflexive)
+    next
+    case (PApp A B)
+      hence "ptrm_subst A z M \<approx> ptrm_subst A z N" and "ptrm_subst B z M \<approx> ptrm_subst B z N"
+        using IH by auto
+      thus ?thesis using PApp ptrm_alpha_equiv.app by auto
+    next
+    case (PFn x T A)
+      consider "x = z" | "x \<noteq> z" by auto
+      thus ?thesis proof(cases)
+        case 1
+          thus ?thesis using PFn by(simp add: ptrm_alpha_equiv_reflexive)
+        next
+        case 2
+          have "\<And>\<pi>. size (\<pi> \<bullet> A) = size A" using ptrm_size_prm by metis
+          hence "\<And>\<pi>. size (\<pi> \<bullet> A) < size (PFn x T A)" by auto
+          hence "\<And>\<pi>. ptrm_subst (\<pi> \<bullet> A) z M \<approx> ptrm_subst (\<pi> \<bullet> A) z N" using IH PFn by metis
+          thus ?thesis
+            using ptrm_alpha_equiv.fn1 PFn `x \<noteq> z` `M \<approx> N` ptrm_alpha_equiv_fvs ptrm_subst.simps(3)
+            by smt
+        next
+      qed
+    next
+  qed
+qed
+
+end
 
 end
